Two pointers with different contents are disjoint

kremlib/C.Nullity.fsti
@@ -36,3 +36,68 @@ let (!*) (#a: Type) (p: pointer a):
   (requires (fun h -> B.live h p))
   (ensures (fun h0 x h1 -> B.live h1 p /\ x == B.get h0 p 0 /\ h1 == h0)) =
   B.index p 0ul
+
+(* TODO: move to FStar.Monotonic.HyperStack *)
+
+private
+let mreference_distinct_sel_disjoint
+  (#a:Type0) (#rel1: Preorder.preorder a) (#rel2: Preorder.preorder a) (h: HS.mem) (r1: HS.mreference a rel1) (r2:HS.mreference a rel2)
+: Lemma
+  (requires (
+    h `HS.contains` r1 /\
+    h `HS.contains` r2 /\
+    HS.frameOf r1 == HS.frameOf r2 /\
+    HS.as_addr r1 == HS.as_addr r2
+  ))
+  (ensures (
+    HS.sel h r1 == HS.sel h r2
+  ))
+= Heap.lemma_distinct_addrs_distinct_preorders ();
+  Heap.lemma_distinct_addrs_distinct_mm ();
+  Heap.lemma_sel_same_addr #a #rel1 (Map.sel h.HS.h (HS.frameOf r1)) (HS.as_ref r1) (HS.as_ref r2)
+
+private
+let mref_distinct_sel_disjoint
+  (#a:Type0) (h: HS.mem) (r1: HS.reference a) (r2: HS.reference a)
+: Lemma
+  (requires (
+    h `HS.contains` r1 /\
+    h `HS.contains` r2 /\
+    HS.frameOf r1 == HS.frameOf r2 /\
+    HS.as_addr r1 == HS.as_addr r2
+  ))
+  (ensures (
+    HS.sel h r1 == HS.sel h r2
+  ))
+= mreference_distinct_sel_disjoint h r1 r2
+
+module U32 = FStar.UInt32
+module Seq = FStar.Seq
+module Heap = FStar.Heap
+
+let pointer_distinct_sel_disjoint
+  (#a: Type)
+  (b1: pointer a)
+  (b2: pointer a)
+  (h: HS.mem)
+: Lemma
+  (requires (
+    B.live h b1 /\
+    B.live h b2 /\
+    B.get h b1 0 =!= B.get h b2 0
+  ))
+  (ensures (
+    B.disjoint b1 b2
+  ))
+= if B.frameOf b1 = B.frameOf b2 && B.as_addr b1 = B.as_addr b2
+  then begin
+    let t1 = B.lseq a (B.max_length b1) in
+    let t2 = B.lseq a (B.max_length b2) in
+    let r1 : HS.reference t1 = B.content b1 in
+    let r2' : HS.reference t2 = B.content b2 in
+    assert (B.max_length b1 == B.max_length b2);
+    assert (t1 == t2);
+    let r2 : HS.reference t1 = r2' in
+    mref_distinct_sel_disjoint h (B.content b1) r2
+  end
+  else ()
